lean/src/r_correct_theorem.lean
@@ -2,9 +2,12 @@ import tactic
 import .a_eval_theorem
 import .defs
 import .helper_defs
+import .leaves
+import data.finset
 
 variable [GuardModule]
 open GuardModule
+variable [decidable_eq Leaf]
 
 local attribute [simp] ant_eval'._match_2
 
@@ -70,7 +73,7 @@ begin
 end
 
 @[simp]
-lemma eval_true_imples_empty_false (is_empty: Gs) { ty: Φ } { env: Env } (h: Φ_eval ty env = tt): is_empty.val ty = ff :=
+lemma eval_true_implies_empty_false (is_empty: Gs) { ty: Φ } { env: Env } (h: Φ_eval ty env = tt): is_empty.val ty = ff :=
 begin
     by_contra,
     have := is_empty.property,
@@ -81,22 +84,24 @@ end
 attribute [simp] R map_ant R'
 local attribute [simp] ant_eval ant_eval' ant_eval_all
 
-lemma r_correct_1 [decidable_eq Leaf]
-    (is_empty: Gs) (gdt: Gdt)
-    
+--(gdt: Gdt)
+--(h_ant: ant_eval ant = some ∘ gdt_eval gdt)
+--(h_leaf: gdt_eval gdt env = Result.leaf leaf):
+--have h: ant_eval ant env = some(Result.leaf leaf), simp [h_ant, h_leaf],
+    --clear h_ant h_leaf,
+
+
+
+
+lemma r_correct_1
+    (is_empty: Gs)    
     (ant: Ant Φ)
-    (h_ant: ant_eval ant = some ∘ gdt_eval gdt)
-    
     (env: Env) (leaf: Leaf)
-    (h_leaf: gdt_eval gdt env = Result.leaf leaf):
+    (h: ant_eval ant env = some (Result.leaf leaf)):
 
         leaf ∈ (R is_empty.val ant).acc
-
     :=
 begin
-    have h: ant_eval ant env = some(Result.leaf leaf), simp [h_ant, h_leaf],
-    clear h_ant h_leaf,
-    
     induction ant generalizing  env,
 
     case Ant.leaf {       
@@ -105,7 +110,7 @@ begin
             finish,
         },
         {
-            have:= eval_true_imples_empty_false is_empty c,
+            have := eval_true_implies_empty_false is_empty c,
             finish,
         }
     },
@@ -133,13 +138,439 @@ begin
             finish,
         },
         finish,
-    }
+    },
+end
+
+@[simp]
+lemma gdt_1 (gdt1: Gdt) (gdt2: Gdt) (env: Env) (h: gdt_eval gdt2 env = Result.no_match):
+            gdt_eval (Gdt.branch gdt1 gdt2) env = gdt_eval gdt1 env :=
+begin
+    rw gdt_eval,
+    cases gdt_eval gdt1 env;
+    finish,
+end
+
+@[simp]
+lemma gdtx (gdt1: Gdt) (gdt2: Gdt) (env: Env) (h: gdt_eval gdt1 env = Result.no_match):
+            gdt_eval (Gdt.branch gdt1 gdt2) env = gdt_eval gdt2 env :=
+begin
+    rw gdt_eval,
+    cases gdt_eval gdt1 env;
+    finish,
+end
+
+lemma gdt_match_1_no_match (gdt: Gdt) (env: Env): gdt_eval._match_1 (Result.no_match) (gdt_eval gdt env) = gdt_eval gdt env :=
+begin
+    cases gdt_eval gdt env;
+    finish,
+end
+
+@[simp]
+lemma gdt_match_branch_match_left (gdt1 gdt2: Gdt) (env: Env) (h: gdt_eval gdt1 env ≠ Result.no_match)
+        : gdt_eval (gdt1.branch gdt2) env = gdt_eval gdt1 env :=
+begin
+    cases c1: gdt_eval gdt1 env;
+    cases c2: gdt_eval gdt2 env;
+    finish [gdt_eval, gdt_eval._match_1],
+end
+
+/-
+@[simp]
+lemma bla2 (gdt: Gdt) (gdt': Gdt) (env: Env) (h: gdt_eval gdt' env = Result.no_match)
+    : gdt_eval._match_1 (gdt_eval gdt env) (gdt_eval gdt' env) = gdt_eval gdt env :=
+begin
+    cases gdt_eval gdt env;
+    finish,
+end
+-/
+
+lemma gdt_branch_replace_left_env { gdt1 gdt1' gdt2: option Gdt } { env: Env }
+    (h: gdt_eval_option gdt1 env = gdt_eval_option gdt1' env):
+    gdt_eval_option (gdt_branch gdt1 gdt2) env = gdt_eval_option (gdt_branch gdt1' gdt2) env :=
+begin
+    cases gdt1;
+    cases gdt1';
+    cases gdt2;
+    
+    finish [gdt_branch, gdt_eval_option, gdt_eval, gdtx],
+end
+
+def 𝒰'option: option Gdt → Φ
+| (some gdt) := 𝒰' gdt
+| none := Φ.true
+
+
+lemma gdt_branch_replace_right_env { gdt1 gdt2 gdt2': option Gdt } { env: Env }
+    (h: (Φ_eval (𝒰'option gdt1) env) → gdt_eval_option gdt2 env = gdt_eval_option gdt2' env):
+    gdt_eval_option (gdt_branch gdt1 gdt2) env = gdt_eval_option (gdt_branch gdt1 gdt2') env :=
+begin
+    cases gdt1,
+    case option.some {
+
+        rw 𝒰'option at h,
+        by_cases c: ↥(Φ_eval (𝒰' gdt1) env),
+        {
+            replace h := h c,
+            replace c := 𝒰_eval1.1 c,
+
+            cases gdt2';
+            cases gdt2;
+            
+            all_goals {
+                try {
+                    simp [gdt_eval_option, gdt_branch, 𝒰'option, gdt_eval, gdt_eval._match_1, c],
+                },
+                try {
+                    simp [gdt_eval_option, gdt_branch, 𝒰'option, gdt_eval, gdt_eval._match_1, c] at h,
+                },
+            },
+            all_goals {
+                exact h,
+            },
+        },
+        {
+            replace c := (not_iff_not.2 𝒰_eval1).1 c,
+            clear h,
+
+            cases gdt2;
+            cases gdt2';
+
+
+            simp [gdt_branch, gdt_eval_option, c],
+        }
+    },
+    case option.none {
+        cases gdt2';
+        cases gdt2;
+        finish [gdt_eval_option, gdt_branch, 𝒰'option],
+    },
 end
 
 
+lemma baz123 { α β: Type } { ant: Ant α } { a1 a2: Ant β } { f: α → β }
+    (h: map_ant f ant = Ant.branch a1 a2):
+    ∃ ant1: Ant α, ∃ ant2: Ant α,
+        ant = Ant.branch ant1 ant2 ∧ a1 = map_ant f ant1 ∧ a2 = map_ant f ant2 :=
+begin
+    cases ant,
+    case Ant.leaf { finish, },
+    case Ant.diverge { finish, },
+    case Ant.branch {
+        rw map_ant at h,
+        use ant_tr1,
+        use ant_tr2,
+        finish,
+    },
+end
+
+--@[simp]
+
+
+lemma R_partition { is_empty: Gs } { ant: Ant Φ } { r: LeafPartition } (h: r = R is_empty.val ant):
+        ant_leaves ant = r.acc.to_finset ∪ r.inacc.to_finset ∪ r.red.to_finset  :=
+begin
+    induction ant generalizing r,
+    case Ant.leaf {
+        simp [ant_leaves, R, map_ant, R'] at h,
+        cases c: is_empty.val ant_a, {
+            simp at c,
+            simp [c] at h,
+            rw h,
+            simp [ant_leaves],
+        }, {
+            simp at c,
+            simp [c] at h,
+            rw h,
+            simp [ant_leaves],
+        },
+    },
+    case Ant.branch {
+        rw ant_leaves,
+        rw [R, map_ant, R'] at h,
+
+        set r1 := R is_empty.val ant_tr1,
+        set r2 := R is_empty.val ant_tr2,
+        replace hr : r = {acc := r1.acc ++ r2.acc, inacc := r1.inacc ++ r2.inacc, red := r1.red ++ r2.red} := h,
+
+        specialize ant_ih_tr1 (refl r1),
+        rw ant_ih_tr1,
+
+        specialize ant_ih_tr2 (refl r2),
+        rw ant_ih_tr2,
+        rw hr,
+
+        simp [finset.union_comm, finset.union_assoc, finset.union_left_comm, to_finset_append],
+    },
+    case Ant.diverge {
+        rw ant_leaves,
+        set r2 := R is_empty.val ant_tr with r2_def,
+        specialize ant_ih (refl r2),
+        
+        let r := R is_empty.val ant_tr,
+        have y := R_diverge ant_a (refl r),
+        cases y,
+        {
+            cases y with rh y,
+            cases y with rs y,
+            cases y with y1 y,
+            
+            finish,
+        },
+        {
+            cases y with y1 y,
+            finish,
+        }
+    },
+end
+
+lemma ant_eval_all_assume_uncovered (gdt: Gdt) (ant: Ant Φ) (env: Env)
+    (h: Φ_eval (𝒰' gdt) env = tt):
+    ant_eval_all (map_ant (𝒰' gdt).and ant) env = ant_eval_all ant env :=
+begin
+    rw ant_eval_all,
+    rw map_ant_associative,
+    rw function.comp,
+    unfold Φ_eval,
+    rw h,
+    simp,
+end
+
+lemma r_correct_2
+    (is_empty: Gs) (gdt: Gdt) (d: disjoint_leaves gdt) (r: LeafPartition) (ant: Ant Φ) (env: Env)
+    (ha: ant_eval_all ant env = ant_eval_all (𝒜' gdt) env)
+    (hr: r = R is_empty.val ant):
+        gdt_eval_option (gdt_remove_leaves r.red.to_finset gdt) env
+        = gdt_eval gdt env :=
+begin
+    induction gdt generalizing r ant,
+
+    case Gdt.leaf {
+
+    },
+
+    case Gdt.branch {
+        -- branch to top
+        rw 𝒜' at ha,
+        rw ant_eval_all at ha,
+        rw ant_eval_all at ha,
+        rw map_ant at ha,
+        rw ←ant_eval_all at ha,
+        rw ←ant_eval_all at ha,
+        rw ←ant_eval_all at ha,
+
+        replace ha := baz123 ha,
+        cases ha with ant1 ha,
+        cases ha with ant2 ha,
+        cases ha with ha1 ha,
+        cases ha with ha2 ha3,
+        rw ←ant_eval_all at ha2,
+        rw ←ant_eval_all at ha3,
+
+
+        rw ha1 at hr,
+        rw R at hr,
+        rw map_ant at hr,
+        rw R' at hr,
+        
+        set r1 := R' (map_ant is_empty.val ant1) with r1_eq,
+        set r2 := R' (map_ant is_empty.val ant2) with r2_eq,
+        replace hr : r = {acc := r1.acc ++ r2.acc, inacc := r1.inacc ++ r2.inacc, red := r1.red ++ r2.red} := hr,
+        
+        rw disjoint_leaves at d,
+        cases d with d_tr1 d,
+        cases d with d_tr2 d,
+        
+
+        specialize gdt_ih_tr1 d_tr1 r1 ant1,
+        replace gdt_ih_tr1 := gdt_ih_tr1 (eq.symm ha2) r1_eq,
+
+
+        rw gdt_remove_leaves,
+ 
+        have grd1_ant1_leaves_eq: ant_leaves ant1 = gdt_leaves gdt_tr1, {
+            rw ←map_leaves_id _ (λ ty, Φ_eval ty env),
+            rw ←ant_eval_all,
+            rw ←ha2,
+            simp [gdt_leaves_eq_ant_leaves, map_leaves_id, ant_eval_all],
+        },
+
+        
+        
+
+
+        have: gdt_remove_leaves r.red.to_finset gdt_tr1 = gdt_remove_leaves r1.red.to_finset gdt_tr1, {
+            rw hr,
+            simp [to_finset_append],
+
+            have: r2.red.to_finset ⊆ ant_leaves ant2, {
+                have x : r2.acc.to_finset ∪ r2.inacc.to_finset ∪ r2.red.to_finset =
+                        r2.red.to_finset ∪ r2.acc.to_finset ∪ r2.inacc.to_finset, {
+                    simp [finset.union_comm, finset.union_assoc, finset.union_left_comm, to_finset_append],
+                },
+                simp [r2.red.to_finset.subset_union_left, R_partition r2_eq, x],
+            },
+            have grd2_ant2_leaves_eq: ant_leaves ant2 = gdt_leaves gdt_tr2, {
+                rw ←map_leaves_id _ (λ ty, Φ_eval ty env),
+                rw ←ant_eval_all,
+                rw ←ha3,
+                simp [gdt_leaves_eq_ant_leaves, map_leaves_id, ant_eval_all],
+            },
+            rw grd2_ant2_leaves_eq at this,
+
+            have: disjoint (gdt_leaves gdt_tr1) r2.red.to_finset, {
+                exact finset.disjoint_of_subset_right this d,
+            },
+
+            have: (r1.red.to_finset ∪ r2.red.to_finset) ∩ gdt_leaves gdt_tr1 = r1.red.to_finset ∩ gdt_leaves gdt_tr1, {
+                rw finset.inter_distrib_right, --(gdt_leaves gdt_tr1) r1.red.to_finset r2.red.to_finset,
+                rw finset.disjoint_iff_inter_eq_empty at this,
+                rw finset.inter_comm at this,
+                simp [this],
+            },
+            
+            rw gdt_remove_leaves_intersect,
+            simp [this, ←gdt_remove_leaves_intersect],
+        },
+
+        rw this,
+
+        have: gdt_eval gdt_tr1 env = gdt_eval_option (some gdt_tr1) env, { simp [gdt_eval_option], },
+
+        rw this at gdt_ih_tr1,
+
+        rw gdt_branch_replace_left_env gdt_ih_tr1,
+
+        clear gdt_ih_tr1,
+        clear this,
+        clear this,
+        clear d_tr1,
+
+
+        
+
+
+        have p: (Φ_eval (𝒰'option (some gdt_tr1)) env) →
+            gdt_eval_option (gdt_remove_leaves r.red.to_finset gdt_tr2) env = gdt_eval_option (some gdt_tr2) env :=
+        begin
+            assume p,
+            rw 𝒰'option at p,
+            rw ant_eval_all at ha3,
+            rw map_ant_associative at ha3,
+            rw function.comp at ha3,
+            unfold Φ_eval at ha3,
+
+            replace p : Φ_eval (𝒰' gdt_tr1) env = tt, exact p,
+            
+            rw p at ha3,
+            simp at ha3,
+            rw ←ant_eval_all at ha3,
+            rw ←ant_eval_all at ha3,
+            rw ←R at r2_eq,
+            specialize gdt_ih_tr2 d_tr2 r2 ant2,
+            replace gdt_ih_tr2 := gdt_ih_tr2 (eq.symm ha3) r2_eq,
+            rw gdt_eval_option,
+            rw ← gdt_ih_tr2,
+            
+            have: gdt_remove_leaves r.red.to_finset gdt_tr2 = gdt_remove_leaves r2.red.to_finset gdt_tr2, {
+                rw hr,
+                simp [to_finset_append],
+
+                have: r1.red.to_finset ⊆ ant_leaves ant1, {
+                    have x : r1.acc.to_finset ∪ r1.inacc.to_finset ∪ r1.red.to_finset =
+                            r1.red.to_finset ∪ r1.acc.to_finset ∪ r1.inacc.to_finset, {
+                        simp [finset.union_comm, finset.union_assoc, finset.union_left_comm, to_finset_append],
+                    },
+                    simp [r1.red.to_finset.subset_union_left, R_partition r1_eq, x],
+                },
+                have grd1_ant1_leaves_eq: ant_leaves ant1 = gdt_leaves gdt_tr1, {
+                    rw ←map_leaves_id _ (λ ty, Φ_eval ty env),
+                    rw ←ant_eval_all,
+                    rw ←ha2,
+                    simp [gdt_leaves_eq_ant_leaves, map_leaves_id, ant_eval_all],
+                },
+                rw grd1_ant1_leaves_eq at this,
+
+                have: disjoint (gdt_leaves gdt_tr2) r1.red.to_finset, {
+                    replace d := disjoint.symm d,
+                    exact finset.disjoint_of_subset_right this d,
+                },
+
+                have: (r1.red.to_finset ∪ r2.red.to_finset) ∩ gdt_leaves gdt_tr2 = r2.red.to_finset ∩ gdt_leaves gdt_tr2, {
+                    rw finset.inter_distrib_right, --(gdt_leaves gdt_tr1) r1.red.to_finset r2.red.to_finset,
+                    rw finset.disjoint_iff_inter_eq_empty at this,
+                    rw finset.inter_comm at this,
+                    simp [this],
+                },
+                
+                rw gdt_remove_leaves_intersect,
+                simp [this, ←gdt_remove_leaves_intersect],
+            },
+            rw this,
+        end,
+
+        rw gdt_branch_replace_right_env p,
+        simp [gdt_branch, gdt_eval_option],
+    },
+end
+
+
+/-
 
 
 
+lemma r_correct_2
+    (is_empty: Gs) (gdt: Gdt) (r: LeafPartition) (ant: Ant Φ)
+    (ha: ant_eval_all ant = ant_eval_all (𝒜' gdt))
+    (hr: r = R is_empty.val ant):
+        gdt_eval_option (gdt_remove_leaves (r.red.remove_all (r.inacc ++ r.acc)) gdt)
+        = gdt_eval gdt :=
+begin
+    induction gdt generalizing r ant,
+
+    case Gdt.branch {
+        ext env:1,
+        replace ha := congr_fun ha env,
+
+        -- branch to top
+        rw 𝒜' at ha,
+        rw ant_eval_all at ha,
+        rw ant_eval_all at ha,
+        rw map_ant at ha,
+        rw ←ant_eval_all at ha,
+        rw ←ant_eval_all at ha,
+        rw ←ant_eval_all at ha,
+
+        replace ha := baz123 ha,
+        cases ha with ant1 ha,
+        cases ha with ant2 ha,
+        cases ha with ha1 ha,
+        cases ha with ha2 ha3,
+        rw ←ant_eval_all at ha2,
+        rw ←ant_eval_all at ha3,
+
+
+        rw ha1 at hr,
+        rw R at hr,
+        rw map_ant at hr,
+        rw R' at hr,
+        
+
+        set r1 := R' (map_ant is_empty.val ant1),
+        set r2 := R' (map_ant is_empty.val ant2),
+        replace hr : r = {acc := r1.acc ++ r2.acc, inacc := r1.inacc ++ r2.inacc, red := r1.red ++ r2.red} := hr,
+        
+        replace ha2: ant_eval_all ant1 = ant_eval_all (𝒜' gdt_tr1) := begin
+            ext env,
+            rw ha2,
+            --library_search,
+        end,
+        specialize gdt_ih_tr1 r1 ant1,
+        rw ← R at r1,
+        
+    },
+end
+    
+-/
 
 
 
@@ -158,7 +589,7 @@ end
 -- Every redundant leaf can be marked as inaccessible instead and
 -- every inaccessible leaf can be marked as accessible instead without invalidating the theorem. This only weakens the analysis.
 
-theorem r_correct [decidable_eq Leaf] : ∀ gdt: Gdt, ∀ is_empty: Gs,
+theorem r_correct : ∀ gdt: Gdt, ∀ is_empty: Gs,
     (
         -- structure + später matchen
         let ⟨ a, i, r ⟩ := ℛ is_empty.val $ 𝒜 gdt
@@ -167,7 +598,7 @@ theorem r_correct [decidable_eq Leaf] : ∀ gdt: Gdt, ∀ is_empty: Gs,
                 -- If all leaves are unique, a, i and r are disjoint.
                 -- In that case, `r.remove_all (i ++ a)` = `r`.
                 -- If all leaves are equal, `r.remove_all (i ++ a)` usually is the empty list.
-                gdt_eval_option (remove_leaves (r.remove_all (i ++ a)) gdt)
+                gdt_eval_option (gdt_remove_leaves (r.remove_all (i ++ a)) gdt)
                 = gdt_eval gdt
             ∧ 
                 -- reachable leaves are accessible.
